\section{Mathematical Showcase}

\begin{theorem}[Pythagoras]
For any right triangle with legs $a,b$ and hypotenuse $c$,
\[
a^2 + b^2 = c^2.
\]
\end{theorem}

\begin{proof}
Consider a right triangle with sides $a$, $b$, and $c$. By construction of squares on each side, the areas satisfy
\[
\text{Area of square on } a + \text{Area of square on } b = \text{Area of square on } c,
\]
hence $a^2 + b^2 = c^2$.
\end{proof}

\begin{theorem}[Sum of the First $n$ Natural Numbers]
\[
\sum_{k=1}^{n} k = \frac{n(n+1)}{2}.
\]
\end{theorem}

\begin{proof}
Consider the sum $S = 1 + 2 + \cdots + n$. Pair terms from opposite ends: $(1+n), (2+n-1), \dots$. Each pair sums to $n+1$, and there are $n/2$ pairs. Thus
\[
S = \frac{n(n+1)}{2}.
\]
\end{proof}

\begin{theorem}[Integral Example]
\[
\int_0^1 x^2 \, dx = \frac{1}{3}.
\]
\end{theorem}

\begin{proof}
\[
\int_0^1 x^2 \, dx = \left[ \frac{x^3}{3} \right]_0^1 = \frac{1}{3}.
\]
\end{proof}

\begin{theorem}[Geometric Series]
For $|r|<1$,
\[
\sum_{k=0}^{\infty} r^k = \frac{1}{1-r}.
\]
\end{theorem}

\begin{proof}
Let $S = 1 + r + r^2 + \cdots$. Then $rS = r + r^2 + r^3 + \cdots$, so
\[
S - rS = 1 \implies S(1-r) = 1 \implies S = \frac{1}{1-r}.
\]
\end{proof}

\begin{theorem}[Quadratic Formula]
For $ax^2 + bx + c = 0$, the solutions are
\[
x = \frac{-b \pm \sqrt{b^2 - 4ac}}{2a}.
\]
\end{theorem}

\begin{proof}
Complete the square:
\[
ax^2 + bx + c = 0 \implies x^2 + \frac{b}{a}x + \frac{c}{a} = 0,
\]
\[
x^2 + \frac{b}{a}x + \left(\frac{b}{2a}\right)^2 = \frac{b^2 - 4ac}{4a^2},
\]
\[
\left(x + \frac{b}{2a}\right)^2 = \frac{b^2 - 4ac}{4a^2} \implies x = \frac{-b \pm \sqrt{b^2 - 4ac}}{2a}.
\]
\end{proof}

\section{Matrices and Determinants}

\[
A = \begin{bmatrix}
1 & 2 & 3 \\
0 & -1 & 4 \\
5 & 6 & 0
\end{bmatrix}, \quad
\det(A) = 1(-1\cdot0 - 4\cdot6) - 2(0\cdot0 - 4\cdot5) + 3(0\cdot6 - (-1)\cdot5) = 9
\]

\section{Multivariable Calculus}

\[
f(x,y) = x^2y + e^y\sin(x), \quad
\frac{\partial f}{\partial x} = 2xy + e^y \cos(x), \quad
\frac{\partial f}{\partial y} = x^2 + e^y \sin(x)
\]

\[
\iint_{[0,1]^2} (x+y) \, dx\, dy = \int_0^1 \int_0^1 (x+y) dx\, dy = \int_0^1 \left[ \frac{x^2}{2} + xy \right]_0^1 dy = \int_0^1 \left( \frac12 + y \right) dy = 1
\]

\section{Limits and Series}

\[
\lim_{n \to \infty} \left( 1 + \frac{1}{n} \right)^n = e
\]

\[
\sum_{n=1}^{\infty} \frac{1}{n^2} = \frac{\pi^2}{6}
\]

\[
\prod_{k=1}^{\infty} \left( 1 + \frac{1}{k^2} \right) = \frac{\sinh(\pi)}{\pi}
\]
