\begin{tcolorbox}[title=Problem 1, breakable]
    \[x^2 + 3x - 2 = 0\]
\end{tcolorbox}

\textbf{Solution:}

\[a = 1, b = 3, c = -2\]
\begin{align*}
    x &= \frac{-b \pm \sqrt{b^2 - 4ac}}{2a} \\
      &= \frac{-3 \pm \sqrt{3^2 - 4(1)(-2)}}{2(1)} \\
      &= \frac{-3 \pm \sqrt{17}}{2}
\end{align*}
So $x = \frac{-3 + \sqrt{17}}{2}$ or $x = \frac{-3 - \sqrt{17}}{2}$.

\begin{tcolorbox}[title=Problem 11, breakable]
    \[x^2 - \sqrt{2}x + 1 = 0\]
\end{tcolorbox}

\[a = 1, b = -\sqrt{2}, c = 1\]
\begin{align*}
    x &= \frac{-b \pm \sqrt{b^2 - 4ac}}{2a} \\
      &= \frac{-(-\sqrt{2}) \pm \sqrt{(-\sqrt{2})^2 - 4(1)(1)}}{2(1)} \\
      &= \frac{\sqrt{2} \pm \sqrt{-2}}{2}
\end{align*}
There are no real solutions.
In $\mathbb{C}$, $x = \frac{\sqrt{2} + \sqrt{-2}}{2}$ or $x = \frac{\sqrt{2} - \sqrt{-2}}{2}$.