\subsection{Equations in Two Unknowns}
\begin{tcolorbox}[title=Problem 7, breakable]
    Solve the following systems of equations for $x$ and $y$.
    \begin{align*}
        7x - y &= 2 \\
        2x + 2y &= 4
    \end{align*}
\end{tcolorbox}

\textbf{Solution 7}
\begin{align*}
    7x - y = 2 \leftrightarrow 14x - 2y = 4 && \\
    (14x - 2y) + (2x + 2y) &= 4 + 4 && \\
    16x &= 8 && \\
    x &= \frac{8}{16} && \\
    x &= \frac{1}{2} && \\ \\
    7x - y &= 2 && \\
    7(\frac{1}{2}) - y &= 2 && \\
    7(\frac{1}{2}) - 2 &= y && \\
    (\frac{7}{2}) - \frac{4}{2} &= y && \\
    \frac{3}{2} &= y
\end{align*}

\begin{tcolorbox}[title=Problem 8, breakable]
    Solve the following systems of equations for $x$ and $y$.
    \begin{align*}
        -4x - 7y &= 5 \\
        2x + y &= 6
    \end{align*}
\end{tcolorbox}

\textbf{Solution 8}
\begin{align*}
    2(2x + y = 6) \leftrightarrow 4x + 2y = 12 && \\
    (4x + 2y) + (-4x - 7y) &= 12 + 5 && \\
    -5y &= 17 && \\
    y &= \frac{-17}{5} && \\ \\
    2x + y &= 6 && \\
    2x + \frac{-17}{5} &= 6 && \\
    2x &= 6  + \frac{17}{5} && \\
    (\frac{10}{5})x &= \frac{30}{5}  + \frac{17}{5} && \\
    (\frac{10}{5})x &= \frac{47}{5} && \\
    x &= \frac{\frac{47}{5}}{(\frac{10}{5})} && \\
    x &= \frac{235}{50} && \\
    x &= \frac{47}{10} && \\
\end{align*}

\begin{tcolorbox}[title=Problem 9, breakable]
    Let $a$, $b$, $c$, $d$ be numbers such that $ad - bc \not = 0$. Solve 
    the following systems of equations for $x$ and $y$ in terms of 
    $a$, $b$, $c$, $d$. \\
    (a) \begin{align*}
            ax + by &= 1 \\
            cx + dy &= 2
        \end{align*}
    (b) \begin{align*}
            ax + by &= 3 \\
            cx + dy &= -4
        \end{align*}
    (c) \begin{align*}
            ax + by &= -2 \\
            cx + dy &= 3 
        \end{align*}
    (d) \begin{align*}
            ax + by &= 5 \\
            cx + dy &= 7
        \end{align*}
\end{tcolorbox}

\textbf{Solution 9 (a)} \\
First multiply by $d$, $ax + by = 1 \leftrightarrow adx + bdy = d$. \\
Then multiply by $b$, $cx + dy = 2 \leftrightarrow bcx + bdy = 2b$. \\
Also multiply by $c$, $ax + by = 1 \leftrightarrow acx + bcy = c$. \\
And mutiply by $a$, $cx + dy  = 2 \leftrightarrow acx + ady = 2a$. 
\begin{align*}
    (adx + bdy) - (bcx + bdy) &= d - 2b && \\
    adx - bcx &= d - 2b && \\
    x(ad - bc) &= d - 2b && \\
    x &= \frac{d - 2b}{ad - bc}
\end{align*}
\begin{align*}
    (acx + ady) - (acx + bcy) &= 2a - c && \\
    ady - bcy &= 2a - c && \\
    y(ad - bc) &= 2a - c && \\
    y(ad - bc) &= \frac{2a - c}{ad - bc} 
\end{align*}

\textbf{Solution 9 (b)} \\
First multiply by $d$, $ax + by = 3 \leftrightarrow adx + bdy = 3d$. \\
Then multiply by $b$, $cx + dy = -4 \leftrightarrow bcx + bdy = -4b$. \\
Also multiply by $c$, $ax + by = 3 \leftrightarrow acx + bcy = 3c$. \\
And mutiply by $a$, $cx + dy  = -4 \leftrightarrow acx + ady = -4a$. 
\begin{align*}
    (adx + bdy) - (bcx + bdy) &= 3d + 4b && \\
    adx - bcx &= 3d + 4b && \\
    x(ad - bc) &= 3d + 4b && \\
    x &= \frac{3d + 4b}{ad - bc}
\end{align*}
\begin{align*}
    (acx + ady) - (acx + bcy) &= -4a - 3c && \\
    ady - bcy &= -4a - 3c && \\
    y(ad - bc) &= -4a - 3c && \\
    y(ad - bc) &= \frac{-4a - 3c}{ad - bc} 
\end{align*}

\textbf{Solution 9 (c)} \\
First multiply by $d$, $ax + by = -2 \leftrightarrow adx + bdy = -2d$. \\
Then multiply by $b$, $cx + dy = 3 \leftrightarrow bcx + bdy = 3b$. \\
Also multiply by $c$, $ax + by = -2 \leftrightarrow acx + bcy = -2c$. \\
And mutiply by $a$, $cx + dy  = 3 \leftrightarrow acx + ady = 3a$. 
\begin{align*}
    (adx + bdy) - (bcx + bdy) &= -2d + 3b && \\
    adx - bcx &= -2d + 3b && \\
    x(ad - bc) &= -2d + 3b && \\
    x &= \frac{-2d + 3b}{ad - bc}
\end{align*}
\begin{align*}
    (acx + ady) - (acx + bcy) &= 3a - c && \\
    ady - bcy &= 3a + 2c && \\
    y(ad - bc) &= 3a + 2c && \\
    y(ad - bc) &= \frac{3a + 2c}{ad - bc} 
\end{align*}

\textbf{Solution 9 (d)} \\
First multiply by $d$, $ax + by = 5 \leftrightarrow adx + bdy = 5d$. \\
Then multiply by $b$, $cx + dy = 7 \leftrightarrow bcx + bdy = 7b$. \\
Also multiply by $c$, $ax + by = 5 \leftrightarrow acx + bcy = 5c$. \\
And mutiply by $a$, $cx + dy  = 7 \leftrightarrow acx + ady = 7a$. 
\begin{align*}
    (adx + bdy) - (bcx + bdy) &= 5d - 7b && \\
    adx - bcx &= 5d - 7b && \\
    x(ad - bc) &= 5d - 7b && \\
    x &= \frac{5d - 7b}{ad - bc}
\end{align*}
\begin{align*}
    (acx + ady) - (acx + bcy) &= 5a - 7c && \\
    ady - bcy &= 5a - 7c && \\
    y(ad - bc) &= 5a - 7c && \\
    y(ad - bc) &= \frac{5a - 7c}{ad - bc} 
\end{align*}

\begin{tcolorbox}[title=Problem 10, breakable]
    Making the same assumptions as in Excersize $9$, show that the solution
    of the system
    \begin{align*}
        ax + by &= 0 && \\
        cx + dy &= 0
    \end{align*}
    must be $x = 0$ and $y = 0$.
\end{tcolorbox}

\textbf{Solution 10} \\
First $ax + by = 0 \leftrightarrow adx + bdy = 0$. \\
Then $cx + dy = 0 \leftrightarrow bcx + bdy = 0$. \\
Also $ax + by = 0 \leftrightarrow acx + bcy = 0$. \\
And $cx + dy = 0 \leftrightarrow acx + ady = 0$. 
\begin{align*}
    (adx + bdy) - (bcx + bdy) &= 0 && \\
    adx - bcx &= 0 && \\
    x(ad - bc) &= 0 && \\
    x &= \frac{0}{ad - bc} \\ 
    x &= 0
\end{align*}
\begin{align*}
    (acx + ady) - (acx + bcy) &= 0 && \\
    ady - bcy &= 0 && \\
    y(ad - bc) &= 0 && \\
    y &= \frac{0}{ad - bc} && \\
    y &= 0
\end{align*}

\begin{tcolorbox}[title=Problem 11, breakable]
    Let $a$, $b$, $c$, $d$, $u$, $v$ be numbers and assume that $ad - bc \not = 0$. 
    Solve the following system of equations for $x$ and $y$ in terms of 
    $a$, $b$, $c$, $d$, $u$, $v$
    \begin{align*}
        ax + by &= u && \\
        cx + dy &= v
    \end{align*}
    Verify that the answer you get is actually a solution.
\end{tcolorbox}


\textbf{Solution 9 (d)} \\
First multiply first equation by $d$, $ax + by = u \leftrightarrow adx + bdy = ud$. \\
Then multiply second equation by $b$, $cx + dy = v \leftrightarrow bcx + bdy = vb$. \\
Also multiply first equation by $c$, $ax + by = u \leftrightarrow acx + bcy = uc$. \\
And multiply second equation by $a$, $cx + dy = v \leftrightarrow acx + ady = va$. 
\begin{align*}
    (adx + bdy) - (bcx + bdy) &= ud - vb && \\
    adx - bcx &= ud - vb && \\
    x(ad - bc) &= ud - vb && \\
    x &= \frac{ud - vb}{ad - bc}
\end{align*}
\begin{align*}
    (acx + ady) - (acx + bcy) &= va - uc && \\
    ady - bcy &= va - uc && \\
    y(ad - bc) &= va - uc && \\
    y &= \frac{va - uc}{ad - bc} && \\
\end{align*}

Veryfying the first equation.

\begin{align*}
    a\left(\frac{ud - vb}{ad - bc}\right) + b\left(\frac{va - uc}{ad - bc}\right) &= u && \\
    \frac{aud - avb + bva - buc}{ad - bc} &= u && \\
    \frac{v(-ab + ba) + u(ad - bc)}{ad - bc} &= u && \\
    \frac{u(ad - bc)}{ad - bc} &= u && \\
    u &= u
\end{align*}

Verifying the second equation.

\begin{align*}
    c\left(\frac{ud - vb}{ad - bc}\right) + d\left(\frac{va - uc}{ad - bc}\right) &= v && \\
    \frac{cud - cvb + dva - duc}{ad - bc} &= v && \\
    \frac{u(cd - cd) + v(ad - bc)}{ad - bc} &= v && \\
    \frac{v(ad - bc)}{ad - bc} &= v && \\
    v &= v
\end{align*}

\subsection{Equations In Three Unknowns}

\begin{tcolorbox}[title=Problem 7, breakable]
    Solve the following equations for $x$, $y$, $z$. \\
    ($1$) $4x - 2y + 5z = 1$ \\
    ($2$) $x + y + z = 0$ \\
    ($3$) $-x + y -2z = 2$
\end{tcolorbox}

\textbf{Solution 7}

Summing ($2$) and ($3$).
\begin{align*}
    (x + y + z) + (-x + y -2z) &= 0 + 2 \\
    \hspace{-2cm}\text{(4)}\quad 2y - z &= 2
\end{align*}
Summing ($1$) and ($2$) multiplied by $-4$.
\begin{align*}
    (4x - 2y + 5z) + (-4x - 4y - 4z) &= 1 + 0 \\
    \hspace{-2cm}\text{(5)}\quad -6y + z &= 1
\end{align*}
Summing ($4$) and ($5$).
\begin{align*}
    (2y - z) + (-6y + z) &= 2 + 1 \\
    -4y &= 3 \\
    y &= \frac{-3}{4}
\end{align*}
Summing ($2$) and ($3$). Setting $y = \frac{-3}{4}$.
\begin{align*}
    (x + \frac{-3}{4} + z) + (-x + \frac{-3}{4} -2z) &= 0 + 2 \\
    2 \cdot \frac{-3}{4} - z &= 2 \\
    \frac{-3}{2} - 2 &= z \\
    \frac{-3}{2} - \frac{4}{2} &= z \\
    \frac{-7}{2} &= z 
\end{align*}
Using ($2$). Setting $y = \frac{-3}{4}$ and $z = \frac{-7}{2}$.
\begin{align*}
    x + \frac{-3}{4} + \frac{-7}{2} &= 0 \\
    x + \frac{-3}{4} + \frac{-14}{4} &= 0 \\
    x + \frac{-17}{4} &= 0 \\
    x &=  \frac{17}{4}
\end{align*}
\[\therefore x =  \frac{17}{4}, y = \frac{-3}{4}, z = \frac{-7}{2} \]

\begin{tcolorbox}[title=Problem 8, breakable]
    Solve the following equations for $x$, $y$, $z$. \\
    ($1$) $x + y + z = 0$ \\
    ($2$) $x - y - z = 1$ \\
    ($3$) $x + y - z = 1$
\end{tcolorbox}

\textbf{Solution 8}

Summing ($1$) and ($2$).
\begin{align*}
    (x + y + z) + (x - y - z) &= 0 + 1 \\
    2x &= 1 \\
    x &= \frac{1}{2} \\
\end{align*}
Summing ($2$) and ($3$). Setting $x = \frac{1}{2}$.
\begin{align*}
    (\frac{1}{2} - y - z) + (\frac{1}{2} + y - z) &= 1 + 1 \\
    1 - 2z &= 2 \\
    -2z &= 1 \\
    z &= \frac{-1}{2} 
\end{align*}
Using ($3$). Setting $x = \frac{1}{2}$ and $z = \frac{-1}{2}$.
\begin{align*}
    \frac{1}{2} + y - (\frac{-1}{2}) &= 1 \\
    y + 1 &= 1 \\
    y &= 0
\end{align*}
\[\therefore x = \frac{1}{2}, y = 0, z = \frac{-1}{2} \]

\begin{tcolorbox}[title=Problem 11, breakable]
    Solve the following equations for $x$, $y$, $z$. \\
    ($1$) $\frac{1}{2}x + y - \frac{3}{4}z = 1$ \\
    ($2$) $x - \frac{1}{2}y + z = 0$ \\
    ($3$) $x + y - \frac{1}{3}z = 0$
\end{tcolorbox}

\textbf{Solution 11}

Multiply ($1$) by $-4$.
\begin{align*}
    \frac{1}{2}x + y - \frac{3}{4}z &= 1 \\
    \hspace{-2cm}\text{(4)}\quad -2x - 4y + 3z &= -4 
\end{align*}
Multiply ($2$) by $2$.
\begin{align*}
    x - \frac{1}{2}y + z &= 0 \\
    \hspace{-2cm}\text{(5)}\quad 2x - y + 2z &= 0
\end{align*}
Multiply ($3$) by $3$.
\begin{align*}
    x + y - \frac{1}{3}z &= 0 \\
    \hspace{-2cm}\text{(6)}\quad 3x + 3y - z &= 0
\end{align*}
Summing ($4$) and ($5$).
\begin{align*}
    (-2x - 4y + 3z) + (2x - y + 2z) &= -4 + 0 \\
    \hspace{-2cm}\text{(7)}\quad -5y + 5z &= -4 
\end{align*}
Sum ($5$) times $3$ and ($6$) times $-2$.
\begin{align*}
    (6x - 3y + 6z) + (-6x - 6y + 2z) &= 0 \\
    \hspace{-2cm}\text{(8)}\quad -9y + 8z &= 0
\end{align*}
Sum ($7$) times $-9$ and ($8$) times $5$.
\begin{align*}
    (45y - 45z) + (-45y + 40z) &= 36 \\
    -5z &= 36 \\
    z &= \frac{-36}{5}
\end{align*}
Using ($7$) and setting $z = \frac{-36}{5}$.
\begin{align*}
    -9y + 8(\frac{-36}{5}) &= 0 \\
    -9y - \frac{288}{5} &= 0 \\
    -9y &= \frac{288}{5} \\
    y &= \frac{-32}{5} \\
\end{align*}
Using ($5$) and setting $y = \frac{-32}{5}$, $z = \frac{-36}{5}$.
\begin{align*}
    2x - (\frac{-32}{5}) + 2(\frac{-36}{5}) &= 0 \\
    2x + \frac{32}{5} - \frac{72}{5} &= 0 \\
    2x - \frac{40}{5}  &= 0 \\
    x &= \frac{40}{10}  \\
    x &= 4 
\end{align*}

\begin{tcolorbox}[title=Problem 12, breakable]
    Solve the following equations for $x$, $y$, $z$. \\
    ($1$) $\frac{1}{2}x - \frac{2}{3}y + z = 1$ \\
    ($2$) $x - \frac{1}{5}y + z = 0$ \\
    ($3$) $2x - \frac{1}{3}y + \frac{2}{5}z = 1$
\end{tcolorbox}

\textbf{Solution 12}

Multiply ($1$) by $6$.
\begin{align*}
    \frac{1}{2}x - \frac{2}{3}y + z &= 1 \\
    \hspace{-2cm}\text{(4)}\quad 3x - 4y + 6z &= 6
\end{align*}
Multiply ($2$) by $-30$.
\begin{align*}
    x - \frac{1}{5}y + z &= 0 \\
    \hspace{-2cm}\text{(5)}\quad -30x + 6y - 30z &= 0
\end{align*}
Multiply ($3$) by $15$.
\begin{align*}
    2x - \frac{1}{3}y + \frac{2}{5}z &= 1 \\
    \hspace{-2cm}\text{(6)}\quad 30x - 5y + 6z &= 15
\end{align*}
Summing ($5$) and ($6$).
\begin{align*}
    (-30x + 6y - 30z) + (30x - 5y + 6z ) &= 15 \\
    \hspace{-2cm}\text{(7)}\quad y - 24z &= 15 
\end{align*}
Sum ($4$) times $10$ and ($5$).
\begin{align*}
    (30x - 40y + 60z) + (-30x + 6y - 30z) &= 60 \\
    \hspace{-2cm}\text{(8)}\quad -34y + 30z &= 60
\end{align*}
Sum ($7$) times $34$ and ($8$).
\begin{align*}
    (34y - 816z) + (-34y + 30z) &= (15 * 34) + 60 \\
    (34y - 816z) + (-34y + 30z) &= 510 + 60 \\
    -786z &= 570 \\
    z &= \frac{-95}{131}
\end{align*}
Using ($7$). Set $z = \frac{-95}{131}$.
\begin{align*}
    y - 24(\frac{-95}{131}) &= 15 \\
    y + \frac{2280}{131} &= 15 \\
    y &= \frac{1965}{131} - \frac{2280}{131} \\
    y &= \frac{-315}{131}
\end{align*}
Using ($7$). Set $z = \frac{-95}{131}$ and $y = \frac{-315}{131}$.
\begin{align*}
    x - \frac{1}{5} \cdot \frac{-315}{131} + \frac{-95}{131} &= 0 \\
    x &=  \frac{1}{5} \cdot \frac{-315}{131} - \frac{-95}{131}  \\
    x &=  \frac{-315}{655} - \frac{-475}{655}  \\
    x &=  \frac{160}{655}  \\
    x &=  \frac{32}{131}
\end{align*}
\[\therefore x = \frac{32}{131}, y = \frac{-315}{131}, z = \frac{-95}{131} \]