\begin{tcolorbox}[title=Problem 1, breakable]
    Find all simultaneous solutions to the Diophantine
    equations $ac - bd = 1$, $ad + bc = 0$ directly,
    by eliminating variables, interpret your solutions 
    as determining all units in the Gaussian integers.
\end{tcolorbox} 

\begin{proof}
    Now, if $c = 0$ then $ad = 0$ implies $a = 0$ or $d = 0$.
    Suppose $a = 0$ then $-bd = 1$ so $b = 1,\ d = -1$
    or $b = -1,\ d = 1$.
    Suppose $d = 0$ then $ac = 1$ so $a = 1,\ c = 1$
    or $a = -1,\ c = -1$.

    Now, suppose $c \ne 0$.
    Then $ad + bc = 0 \iff bc = -ad \iff b = -\frac{ad}{c}$.
    Plugging in we find
    $$
    ac - \left(-\frac{ad}{c}\right)d = 1
    \iff ac + \frac{ad^2}{c} = 1
    \iff a(c^2 + d^2) = c
    \iff a = \frac{c}{c^2 + d^2}.
    $$
    Which only has solutions $c^2 + d^2 = 1$.

    Thus the solutions are $a = \pm 1,\ b = 0,\ c = \pm 1,\ d = 0$
    or $a = 0,\ b = \pm 1,\ c = 0,\ d = \pm 1$.
\end{proof}

\begin{tcolorbox}[title=Problem 2, breakable]
    Prove Theorem 10.1. That is, let $n$, be a square-free integer.
    As in the text, define $N(a + b\sqrt{n}) = |a^2 - nb^2|$.
    Prove that $N$ preserves multiplication, that is,
    $N(\alpha \beta) = N(\alpha) N(\beta)$.
\end{tcolorbox} 

\begin{proof}
    Let $\alpha = a + b\sqrt{n}$ and $\beta = c + d\sqrt{n}$.
    Then
    \[
    N(\alpha \beta)
        = N((a + b\sqrt{n})(c + d\sqrt{n}))
        = N(ac + ad\sqrt{n} + bc\sqrt{n} + bdn)
    \]
    \[
        = N((ac + bdn) + (ad + bc)\sqrt{n})
        = |(ac + bdn)^2 - n(ad + bc)^2|.
    \]
    Similarly
    \[
    N(\alpha)N(\beta)
        = N(a + b\sqrt{n})N(c + d\sqrt{n})
        = |a^2 - nb^2||c^2 - nd^2|.
    \]
    Then
    \[
    (ac + bdn)^2 - n(ad + bc)^2
    = a^2c^2 + 2abcd\,n + b^2d^2n^2
    - n(a^2d^2 + 2abcd + b^2c^2),
    \]
    which simplifies to
    \[
    a^2c^2 - na^2d^2 - nb^2c^2 + n^2b^2d^2.
    \]
    Then
    \[
    (a^2 - nb^2)(c^2 - nd^2)
    = a^2c^2 - na^2d^2 - nb^2c^2 + n^2b^2d^2.
    \]
    Thus $N(\alpha\beta) = N(\alpha)N(\beta)$.
\end{proof}

\begin{tcolorbox}[title=Problem 3, breakable]
    Suppose that $n, m$ are distinct square-free integers.
    Prove that $\mathbb{Z}[\sqrt{n}] \cap \mathbb{Z}[\sqrt{m}] = \mathbb{Z}$.
    This is not true if at least one of the integers $n$ and $m$ is not 
    square-free. Give an example to show this.
\end{tcolorbox} 


\begin{theorem}
    Suppose $n, m$ are square free integers such that $n \ne m$ and $a, b \in \mathbb{Z}$.
    Futhermore, suppose $a \ne 0, b \ne 0$ and $x = a\sqrt{n} - b\sqrt{m}$.
    Then $x$ is an irrational number.
\end{theorem}

\begin{proof}
    For contradiction, suppose $x$ is rational.
    Then $x = a\sqrt{n} - b \sqrt{m} \iff x + b\sqrt{m} = a \sqrt{n} \iff \frac{x + b\sqrt{m}}{a} = \sqrt{n}$.
    Now squaring both sides we find $\frac{x^2 + 2xb\sqrt{m} + b^2 m}{a^2} = n \iff x^2 + 2xb\sqrt{m} + b^2 m = a^2 n \iff 2xb\sqrt{m} = a^2 n - x^2 - b^2 m$.
    Now the rhs is an integer but the lhs is irrational which is a contradiction.
\end{proof}

\begin{proof}
    Let $x$ be an arbitrary element in $\mathbb{Z}[\sqrt{n}] \cap \mathbb{Z}[\sqrt{m}]$.
    Then $x = a + b\sqrt{n}$ and $x = c + d\sqrt{m}$ for some $a, b, c, d \in \mathbb{Z}$.
    Then $a + b\sqrt{n} = c + d\sqrt{m} \iff b\sqrt{n} - d\sqrt{m} = c - a$. 
    Now the lhs is irrational unless $b = d = 0$.
    Thus $a = c$ and $x \in \mathbb{Z}$.
    Conversely, any integer $z \in \mathbb{Z}$ is in both $\mathbb{Z}[\sqrt{n}]$ and $\mathbb{Z}[\sqrt{m}]$,
    so $\mathbb{Z} \subseteq \mathbb{Z}[\sqrt{n}] \cap \mathbb{Z}[\sqrt{m}]$.
    Thus, $\mathbb{Z}[\sqrt{n}] \cap \mathbb{Z}[\sqrt{m}] = \mathbb{Z}$.
\end{proof}

\begin{proof}
    Let $n = 2$ and $m = 8$.
    Then $\sqrt{8} = 2\sqrt{2}$ and thus $\mathbb{Z}[\sqrt{2}] = \mathbb{Z}[\sqrt{8}]$.
    Therefore,
    \[
        \mathbb{Z}[\sqrt{2}] \cap \mathbb{Z}[\sqrt{8}] = \mathbb{Z}[\sqrt{2}] \neq \mathbb{Z}.
    \]
\end{proof}

\begin{tcolorbox}[title=Problem 4, breakable]
    Prove that the Diophantine equation $2b^2 = a^2 + 3$ has no 
        integer solutions, proceeding similarly as the problem 
        $a^2 = 2b^2 + 3$ is handled in the text in Example 10.16.
\end{tcolorbox} 

\begin{proof}
    Now $2b^2 = a^2 + 3 \iff a^2 = 2b^2 - 3$, thus $a$ is odd
        and can be written as $2k_1 + 1$ with $k_1 \in \mathbb{Z}$.
    Then $(2k_1 + 1)^2 = 2b^2 - 3 \iff 4 k_1^2 + 4k_1 + 1 = 2b^2 - 3 \iff 2(2k_1^2 + 2k_1 + 2) = 2b^2$.
    Thus $b^2 = 2k_1^2 + 2k_1 + 2$, so $b$ is even and can be written as $2k_2$ for some $k_2 \in \mathbb{Z}$.
    Substituting, we obtain $2(2k_2)^2 = a^2 + 3 \iff 2k_2^2 = k_1^2 + 1$.
    But this equation has the same form as the original with smaller positive integers.
    Repeating this process contradicts the well-ordering principle for positive integers,
     and thus there are no integer solutions.
\end{proof}

\begin{tcolorbox}[title=Problem 5 breakable]
    Find infinitely many distinct units in $\mathbb{Z}[\sqrt{7}]$. 
    Then list inifintely many associates of $\sqrt{7}$ in $\mathbb{Z}[\sqrt{7}]$.
\end{tcolorbox} 
